lib/Trace_Schematic_Insts: refactor; improve ML style

lib/Trace_Schematic_Insts.thy
@@ -25,148 +25,174 @@ text \<open>
   (for now, we don't worry about types that don't have sort "type").
 
   TODO: there ought to be some standard way of stashing things into
-  the proof goal. Find out what that is and refactor
+  the proof state. Find out what that is and refactor
 \<close>
-definition trace_schematic_insts__container :: "'a \<Rightarrow> bool \<Rightarrow> bool"
+definition proof_state_term__container :: "'a \<Rightarrow> bool \<Rightarrow> bool"
   where
-  "trace_schematic_insts__container a b \<equiv> True"
+  "proof_state_term__container a b \<equiv> True"
 
-lemma trace_schematic_insts__container_add:
-  "Pure.prop PROP P \<equiv> PROP Pure.prop (trace_schematic_insts__container True xs \<Longrightarrow> PROP P)"
-  by (simp add: trace_schematic_insts__container_def)
+lemma proof_state_term__container_add:
+  "Pure.prop PROP P \<equiv> PROP Pure.prop (proof_state_term__container True xs \<Longrightarrow> PROP P)"
+  by (simp add: proof_state_term__container_def)
 
-lemma trace_schematic_insts__container_remove:
-  "PROP Pure.prop (trace_schematic_insts__container True xs \<Longrightarrow> PROP P) \<equiv> Pure.prop (PROP P)"
-  by (simp add: trace_schematic_insts__container_def)
+lemma proof_state_term__container_remove:
+  "PROP Pure.prop (proof_state_term__container True xs \<Longrightarrow> PROP P) \<equiv> Pure.prop (PROP P)"
+  by (simp add: proof_state_term__container_def)
 
 ML \<open>
-structure Trace_Schematic_Insts = struct
+signature TRACE_SCHEMATIC_INSTS = sig
+  val trace_schematic_insts:
+        Method.method -> ((term * term) list -> (typ * typ) list -> unit) -> Method.method
+  val default_report:
+        Proof.context -> string -> (term * term) list -> (typ * typ) list -> unit
+
+  val skip_dummy_state: Method.method -> Method.method
+  val make_term_container: term list -> term
+  val dest_term_container: term -> term list
+  val attach_proof_annotations: Proof.context -> term list -> thm -> thm
+  val detach_proof_annotations: Proof.context -> thm -> term list * thm
+end
+
+structure Trace_Schematic_Insts: TRACE_SCHEMATIC_INSTS = struct
 
 (* Work around Isabelle running every apply method on a dummy proof state *)
-fun skip_dummy_state (method: Method.method) : Method.method =
+fun skip_dummy_state method =
   fn facts => fn (ctxt, st) =>
     case Thm.prop_of st of
-        Const ("Pure.prop", _) $ (Const ("Pure.term", _) $ Const ("Pure.dummy_pattern", _)) =>
+        Const (@{const_name Pure.prop}, _) $
+          (Const (@{const_name Pure.term}, _) $ Const (@{const_name Pure.dummy_pattern}, _)) =>
           Seq.succeed (Seq.Result (ctxt, st))
       | _ => method facts (ctxt, st);
 
 (* Utils *)
-fun rewrite_state_concl (eqn: thm) (st: thm) : thm =
+fun rewrite_state_concl eqn st =
   Conv.fconv_rule (Conv.concl_conv (Thm.nprems_of st) (K eqn)) st
 
 (* Strip the @{term Prop.prop} that wraps proof state conclusions *)
-fun strip_prop (ct: cterm): cterm = case Thm.term_of ct of
-        Const ("Pure.prop", @{typ "prop \<Rightarrow> prop"}) $ _ => Thm.dest_arg ct
+fun strip_prop ct =
+      case Thm.term_of ct of
+        Const (@{const_name "Pure.prop"}, @{typ "prop \<Rightarrow> prop"}) $ _ => Thm.dest_arg ct
       | _ => raise CTERM ("strip_prop: head is not Pure.prop", [ct])
 
-fun cconcl_of (st: thm): cterm =
+fun cconcl_of st =
   funpow (Thm.nprems_of st) Thm.dest_arg (Thm.cprop_of st)
   |> strip_prop
 
-fun vars_of_term (t: term): (indexname * typ) list =
+fun vars_of_term t =
   Term.add_vars t []
   |> sort_distinct Term_Ord.var_ord
 
-fun type_vars_of_term (t: term): (indexname * sort) list =
+fun type_vars_of_term t =
   Term.add_tvars t []
   |> sort_distinct Term_Ord.tvar_ord
 
 (* Create annotation list *)
-fun make_schematics_container ts =
+fun make_term_container ts =
       fold (fn t => fn container =>
-              Const (@{const_name trace_schematic_insts__container},
+              Const (@{const_name proof_state_term__container},
                     fastype_of t --> @{typ "bool \<Rightarrow> bool"}) $
                 t $ container)
         (rev ts) @{term "True"}
 
 (* Retrieve annotation list *)
-fun dest_schematics_container
-      (Const (@{const_name trace_schematic_insts__container}, _) $ @{term True} $ list) =
-      let fun dest (Const (@{const_name trace_schematic_insts__container}, _) $ x $ list) =
-                x :: dest list
-            | dest _ = []
-      in dest list end
-  | dest_schematics_container t =
-      raise TERM ("Trace_Schematic_Insts internal error: not a schematic container", [t])
+fun dest_term_container
+      (Const (@{const_name proof_state_term__container}, _) $ x $ list) =
+          x :: dest_term_container list
+  | dest_term_container _ = []
+
+(* Attach some terms to a proof state *)
+fun attach_proof_annotations ctxt terms st =
+  let
+    val container = make_term_container terms
+    (* FIXME: this might affect st's maxidx *)
+    val add_eqn =
+          Thm.instantiate
+            ([],
+             [((("P", 0), @{typ prop}), cconcl_of st),
+              ((("xs", 0), @{typ bool}), Thm.cterm_of ctxt container)])
+            @{thm proof_state_term__container_add}
+  in
+    rewrite_state_concl add_eqn st
+  end
+
+(* Retrieve attached terms from a proof state *)
+fun detach_proof_annotations ctxt st =
+  let
+    val st_concl = cconcl_of st
+    val (ccontainer', real_concl) = Thm.dest_implies st_concl
+    val ccontainer =
+          ccontainer'
+          |> Thm.dest_arg (* strip Trueprop *)
+          |> Thm.dest_arg (* strip outer "p_s_t__c True" *)
+    val terms =
+          ccontainer
+          |> Thm.term_of
+          |> dest_term_container
+    val remove_eqn =
+          Thm.instantiate
+            ([],
+             [((("P", 0), @{typ prop}), real_concl),
+              ((("xs", 0), @{typ bool}), ccontainer)])
+            @{thm proof_state_term__container_remove}
+  in
+    (terms, rewrite_state_concl remove_eqn st)
+  end
 
 (* ML interface, calls the supplied function with schematic unifications
    (will be given all variables, including those that haven't been instantiated) *)
-fun trace_schematic_insts
-      (method: Method.method)
-      (callback: (term * term) list -> (typ * typ) list -> unit)
-  : Method.method
+fun trace_schematic_insts method callback
   = fn facts => fn (ctxt, st) =>
     let val tvars = map TVar (type_vars_of_term (Thm.prop_of st))
         val tvar_carriers = map (fn tvar => Const (@{const_name undefined}, tvar)) tvars
         val vars = map Var (vars_of_term (Thm.prop_of st))
-        val container = make_schematics_container (vars @ tvar_carriers)
-
-        (* FIXME: this might affect st's maxidx *)
-        val add_schematics_eqn = Thm.instantiate
-              ([],
-               [((("P", 0), @{typ prop}), cconcl_of st),
-                ((("xs", 0), @{typ bool}), Thm.cterm_of ctxt container)])
-              @{thm trace_schematic_insts__container_add}
-        (* Now stash it into st *)
-        val annotated_st = rewrite_state_concl add_schematics_eqn st
+        val annotated_st = attach_proof_annotations ctxt (vars @ tvar_carriers) st
     in (* Run the method *)
-       method facts (ctxt, annotated_st)
-       |> Seq.map_result (fn (ctxt', annotated_st') => let
-            val st'_concl = cconcl_of annotated_st'
+      method facts (ctxt, annotated_st)
+      |> Seq.map_result (fn (ctxt', annotated_st') => let
             (* Retrieve the stashed list, now with unifications *)
-            val st'_annotations =
-                  st'_concl
-                  |> Thm.dest_implies |> fst
-                  |> Thm.dest_arg (* strip Trueprop *)
-            val container' = Thm.term_of st'_annotations |> dest_schematics_container
-            val (var_annotations, tvar_annotations) = chop (length vars) container'
+            val (annotations, st') = detach_proof_annotations ctxt' annotated_st'
+            val (var_annotations, tvar_annotations) = chop (length vars) annotations
             (* Report the list *)
             (* TODO: provide attached Bounds as well? *)
             val _ = callback (vars ~~ var_annotations) (tvars ~~ map fastype_of tvar_annotations)
-
-            (* Restore original conclusion of st *)
-            val st'_real_concl =
-                  st'_concl
-                  |> Thm.dest_implies |> snd
-            val dest_schematics_eqn = Thm.instantiate
-                  ([],
-                   [((("P", 0), @{typ prop}), st'_real_concl),
-                    ((("xs", 0), @{typ bool}),
-                     Thm.dest_arg st'_annotations (* strip outer "t_s_i__c True" *))])
-                  @{thm trace_schematic_insts__container_remove}
-            val st' = rewrite_state_concl dest_schematics_eqn annotated_st'
-       in (ctxt', st') end)
+         in (ctxt', st') end)
     end
+
+(* Default callback. Prints nontrivial instantiations to tracing output
+   with the given title line *)
+fun default_report ctxt title var_insts tvar_insts =
+  let
+    val vars_lines =
+        map (fn (var, inst) =>
+          if var = inst then "" (* don't show unchanged *) else
+              "  " ^ Syntax.string_of_term ctxt var ^ "  =>  " ^
+              Syntax.string_of_term ctxt inst ^ "\n")
+        var_insts
+    val tvars_lines =
+        map (fn (tvar, inst) =>
+          if tvar = inst then "" (* don't show unchanged *) else
+              "  " ^ Syntax.string_of_typ ctxt tvar ^ "  =>  " ^
+              Syntax.string_of_typ ctxt inst ^ "\n")
+        tvar_insts
+    val all_insts = String.concat (vars_lines @ tvars_lines)
+  (* TODO: add a quiet flag, to suppress output when nothing was instantiated *)
+  in title ^ "\n" ^ (if all_insts = "" then "  (no instantiations)\n" else all_insts)
+     |> tracing
+  end
 end
 \<close>
 
 method_setup trace_schematic_insts = \<open>
   let
-    fun show_insts ctxt title var_insts tvar_insts = let
-        val vars_lines =
-            map (fn (var, inst) =>
-              if var = inst then "" (* don't show unchanged *) else
-                  "  " ^ Syntax.string_of_term ctxt var ^ "  =>  " ^
-                  Syntax.string_of_term ctxt inst ^ "\n")
-            var_insts
-        val tvars_lines =
-            map (fn (tvar, inst) =>
-              if tvar = inst then "" (* don't show unchanged *) else
-                  "  " ^ Syntax.string_of_typ ctxt tvar ^ "  =>  " ^
-                  Syntax.string_of_typ ctxt inst ^ "\n")
-            tvar_insts
-        val all_insts = String.concat (vars_lines @ tvars_lines)
-        (* TODO: add a quiet flag, to suppress output when nothing was instantiated *)
-        in title ^ "\n" ^ (if all_insts = "" then "  (no instantiations)\n" else all_insts)
-           |> tracing
-        end
+    open Trace_Schematic_Insts
   in
     (Scan.option (Scan.lift Parse.liberal_name) -- Method.text_closure) >>
     (fn (maybe_title, method_text) => fn ctxt =>
-      Trace_Schematic_Insts.trace_schematic_insts
+      trace_schematic_insts
           (Method.evaluate method_text ctxt)
-          (show_insts ctxt (Option.getOpt (maybe_title, "trace_schematic_insts:")))
-      |> Trace_Schematic_Insts.skip_dummy_state
+          (default_report ctxt
+              (Option.getOpt (maybe_title, "trace_schematic_insts:")))
+      |> skip_dummy_state
     )
   end
 \<close> "Method combinator to trace schematic variable and type instantiations"
